io/IIO.Behavior.fst
@@ -6,6 +6,8 @@ open FStar.FunctionalExtensionality
 open BeyondCriteria
 open IIO
 
+(** reify is not implemented in F* *)
+(** our reify is ghost because we want to use it only when reasoning *)
 assume val __reify_IIOwp (#a:Type) (#wp:Hist.hist a) (#fl:tflag) ($f:unit -> IIOwp a fl wp) : GTot (dm_giio a fl wp)
 
 (** Confusing elements:
@@ -13,7 +15,18 @@ assume val __reify_IIOwp (#a:Type) (#wp:Hist.hist a) (#fl:tflag) ($f:unit -> IIO
 2) prefixed_trace_property may be confusing 
 **)
 
-type prefixed_trace_property (pre:IIO.Sig.trace -> Type0) = h:IIO.Sig.trace -> (#_:squash (pre h)) -> BeyondCriteria.trace #event -> Type0
+(** The idea of prefixed_trace_property comes from the need to reason 
+about the behavior of contexts. When reasoning about contexts,
+we have to take in account that the context is called by the partial
+program which already produced some events --- that can affect the 
+behavior of the context / the instrumentation **)
+type prefixed_trace_property (pre:IIO.Sig.trace -> Type0) = 
+  h:IIO.Sig.trace -> (#_:squash (pre h)) -> BeyondCriteria.trace #event -> Type0
+
+type prefixed_trace (pre:trace->Type0) = h:trace{pre h} * BeyondCriteria.trace #event  
+
+let pt_mem (#pre:trace->Type0) ((h, tr):prefixed_trace pre) (s1:prefixed_trace_property pre) =
+  s1 h tr
 
 (* We define `beh_giio` that returns the set of traces produced by a program
    starting from a given history `h`.
@@ -36,6 +49,7 @@ val _beh : (unit -> IIO int AllActions (fun _ -> True) (fun _ _ _ -> True)) -> t
 let _beh ws =
   beh_giio (__reify_IIOwp ws) []
 
+(** used for whole programs **)
 irreducible
 val beh : (unit -> IIO int AllActions (fun _ -> True) (fun _ _ _ -> True)) ^-> trace_property #event
 let beh = on_domain _ (fun ws -> _beh ws)
@@ -44,52 +58,7 @@ val _beh_ctx : #pre:(trace -> Type0) -> (unit -> IIO int AllActions pre (fun _ _
 let _beh_ctx ws h =
   beh_giio (__reify_IIOwp ws) h 
 
+(** used for contexts **)
 //irreducible
 val beh_ctx : #pre:(trace -> Type0) -> (unit -> IIO int AllActions pre (fun _ _ _ -> True)) ^-> prefixed_trace_property pre 
 let beh_ctx #pre = on_domain _ (fun ws -> _beh_ctx #pre ws)
-
-type prefixed_trace (pre:trace->Type0) = h:trace{pre h} * BeyondCriteria.trace #event  
-
-let mem (#pre:trace->Type0) ((h, tr):prefixed_trace pre) (s1:prefixed_trace_property pre) =
-  s1 h tr
-
-open FStar.Tactics
-
-val lemma0 : #pre:(trace -> Type0) -> ctx:(fl:erased tflag -> unit -> IIO int fl pre (fun _ _ _ -> True)) -> h1:trace{pre h1} -> h2:trace{pre h2} -> tr:BeyondCriteria.trace -> Lemma (
-  let reified_ctx = __reify_IIOwp (ctx AllActions) in
-  beh_giio #pre reified_ctx h1 tr ==> beh_giio #pre reified_ctx h2 tr
-)
-
-let lemma0 #pre ctx h1 h2 tr =
-  let reified_ctx = __reify_IIOwp (ctx AllActions) in
-  introduce beh_giio #pre reified_ctx h1 tr 
-  ==> beh_giio #pre reified_ctx h2 tr 
-  with _. begin
-    assume (beh_giio #pre reified_ctx h2 tr)
-  end
-
-(* h is non-interfering for flag polymorphic ctx
-  -- should be true since a flag polymorphic ctx can do no actions *)
-val test : #pre:(trace -> Type0) -> ctx:(fl:erased tflag -> unit -> IIO int fl pre (fun _ _ _ -> True)) ->
-  Lemma (
-    let bh = beh_ctx #pre (ctx AllActions) in
-    forall t1 t2. t1 `mem` bh /\ t2 `mem` bh ==>
-      (exists t3. t3 `mem` bh /\ fst t1 == fst t3 /\ snd t2 == snd t3))
-
-let test #pre ctx = 
-  let bh = beh_ctx #pre (ctx AllActions) in
-  let reified_ctx : dm_giio int AllActions (to_hist pre (fun _ _ _ -> True)) = __reify_IIOwp (ctx AllActions) in
-  introduce forall (t1 t2:prefixed_trace pre).
-  t1 `mem` bh /\ t2 `mem` bh 
-  ==> (exists (t3:prefixed_trace pre). t3 `mem` bh /\ fst t1 == fst t3 /\ snd t2 == snd t3) 
-  with begin
-    introduce t1 `mem` bh /\ t2 `mem` bh
-    ==> (exists (t3:prefixed_trace pre). t3 `mem` bh /\ fst t1 == fst t3 /\ snd t2 == snd t3)
-    with _. begin
-      let t3 : prefixed_trace pre = (fst t1, snd t2) in 
-      assert (t2 `mem` bh);
-      lemma0 #pre ctx (fst t2) (fst t1) (snd t2);
-      assert (beh_giio #pre reified_ctx (fst t2) (snd t2) ==> beh_giio #pre reified_ctx (fst t1) (snd t2));
-      assert (t3 `mem` bh)
-    end
-  end
